Lambda.dfy
@@ -1,0 +1,141 @@
+include "objects.dfy"
+type Id= string 
+datatype LambdaTerm = Var(name:string) | Lambda(x:Id,t:LambdaTerm) | Application( t1:LambdaTerm, t2:LambdaTerm)
+
+function bound(t:LambdaTerm):seq<Id>
+    ensures allUnique(bound(t))
+{
+        match t
+                case Var(_) => []
+                case Lambda(x,t) => addition(x,bound(t))
+                case Application(t1,t2) => reunion(bound(t1),bound(t2))
+}
+function addition(x:Id,s:seq<Id>) : seq<Id>
+    requires allUnique(s)
+    ensures var s':=addition(x,s);
+            allUnique(s') && x in s'
+{
+    if x in s then s
+    else  assert !(x in s);
+        assert x in (s+[x]);
+        assert allUnique(s+[x]); 
+        s+[x]
+}
+function reunion(s1:seq<Id>,s2:seq<Id>) :seq<Id>
+    requires allUnique(s1)
+    requires allUnique(s2)
+    ensures var s:=reunion(s1,s2);
+        allUnique(s) 
+        && (forall str:Id::str in s ==> (str in s1 || str in s2))
+        && (forall str:Id::str in s1 || str in s2 ==> (str in s) )&&
+        |s| >= |s1| && |s| >= |s2|
+{
+    if s1==[] 
+        then s2
+    else
+
+        [s1[0]]+reunion(remove(s1,s1[0]),remove(s2,s1[0]))
+}
+lemma elementNotInallUnique (s:seq<Id>,x:Id)
+    requires !(x in s)
+    requires allUnique(s)
+    ensures allUnique([x]+s)
+{
+}    
+ghost predicate allUnique (s:seq<Id>) 
+{
+    forall id1:nat,id2:nat::(id1<id2<|s|) ==> s[id1]!=s[id2]
+}
+ghost predicate isGoodForWork(s:seq<Id>)
+    requires allUnique(s)
+{
+    forall str:Id:: ((str in s) && |str|>1 && str[0]=='n' && isStringAValidNumber(str[1..])) ==> stringToNat(str[1..])<|s|
+}
+lemma reunionIsGoodForWork(s1:seq<Id>,s2:seq<Id>)
+    requires allUnique(s1) && isGoodForWork(s1)
+    requires allUnique(s2) && isGoodForWork(s2)
+    ensures allUnique(reunion(s1,s2)) && isGoodForWork(reunion(s1,s2))
+{
+    var s:=reunion(s1,s2);
+    assert forall str:Id::(str in s1 || str in s2) ==> (str in s);
+    assert forall str:Id::str in s1 ==> (str in s);
+    assert |s|>=|s1|;
+    assert |s|>=|s1| && |s|>=|s2|;
+}
+function addAnUniqueId(s:seq<Id>) : seq<Id>
+    requires allUnique(s) && isGoodForWork(s)
+    ensures allUnique(addAnUniqueId(s)) && isGoodForWork(addAnUniqueId(s))
+{
+    var str:="n"+natToString(|s|);
+    natToStringThenStringToNatIdem(|s|);
+    assert !(str in s);
+    [str] +s
+}
+function remove(s:seq<Id>,x:Id):seq<Id>
+    requires allUnique(s) 
+    ensures ! (x in remove(s,x))
+    ensures allUnique(remove(s,x))
+    ensures forall str:Id:: str in remove(s,x) ==> str in s
+    ensures forall str:Id:: str in s && str!=x ==> str in remove(s,x)
+    ensures |s|-1<=|remove(s,x)|<=|s|
+{
+    if s==[] then []
+    else 
+        if   
+            s[0]==x then s[1..]
+        else 
+        assert allUnique(remove(s[1..],x));
+        assert ! (s[0] in remove(s[1..],x));
+        elementNotInallUnique(remove(s[1..],x),s[0]);
+        [s[0]]+remove(s[1..],x)
+
+}
+function free(t:LambdaTerm):seq<Id>
+    ensures allUnique(free(t))
+{
+     match t
+                case Var(x) => [x]
+                case Lambda(x,t) => remove(free(t),x)
+                case Application(t1,t2) => reunion(free(t1),free(t2))
+}
+
+function vars(t:LambdaTerm):seq<Id>
+    ensures allUnique(vars(t))
+{
+    match t
+                case Var(x) => [x]
+                case Lambda(x,t') => addition(x,vars(t'))
+                case Application(t1,t2) => reunion(vars(t1),vars(t2))
+}
+function substitution(t:LambdaTerm,x:Id,t':LambdaTerm):LambdaTerm
+{
+    match t
+        case Var(y) => if y==x then t' else Var(y)
+        case Lambda(y,t1) => if y==x then t else   Lambda(y,substitution(t1,x,t'))
+        case Application(t1,t2) => Application(substitution(t1,x,t'),substitution(t2,x,t'))
+}
+
+function caSubstitution(t:LambdaTerm,x:Id,t':LambdaTerm):LambdaTerm
+    requires var s1:=vars(t);
+        allUnique(s1) && isGoodForWork(s1)
+    requires var s2:=vars(t');
+        allUnique(s2) && isGoodForWork(s2)
+    ensures var s:=vars(caSubstitution(t,x,t'));
+        allUnique(s) && isGoodForWork(s)
+{
+    caSubstitution'(t,x,t',reunion(vars(t),vars(t')))
+}
+
+function caSubstitution'(t:LambdaTerm,x:Id,t':LambdaTerm,ids:seq<Id>):LambdaTerm
+    requires forall str:Id::str in reunion(vars(t),vars(t')) ==> str in ids 
+    requires allUnique(ids) && isGoodForWork(ids)
+{
+    match t
+        case Var(y) => if y==x then t' else Var(y)
+        case Lambda(y,t1) => if y==x then t else
+                                if !(y in free(t')) then Lambda(y,caSubstitution'(t,x,t',ids))
+                                    else
+                                        var ids':=addAnUniqueId(ids);
+                                        Lambda(ids'[0],caSubstitution'())
+        case Application(t1,t2) => Application(substitution(t1,x,t'),substitution(t2,x,t'))
+}
